examples/ghc/theories/CoreSubstInvariants.v
@@ -1,0 +1,106 @@
+Require Import CoreSyn.
+Require Import Id.
+Require Import IdInfo.
+Require Import VarSet.
+Require Import BasicTypes.
+
+Require Import Coq.Lists.List.
+Require Import Coq.Bool.Bool.
+Require Import Coq.ZArith.BinInt.
+
+Set Bullet Behavior "Strict Subproofs".
+
+(*
+-- | A substitution environment, containing 'Id', 'TyVar', and 'CoVar'
+-- substitutions.
+--
+-- Some invariants apply to how you use the substitution:
+--
+-- 1. #in_scope_invariant# The in-scope set contains at least those 'Id's and 'TyVar's that will be in scope /after/
+-- applying the substitution to a term. Precisely, the in-scope set must be a superset of the free vars of the
+-- substitution range that might possibly clash with locally-bound variables in the thing being substituted in.
+--
+-- 2. #apply_once# You may apply the substitution only /once/
+--
+-- There are various ways of setting up the in-scope set such that the first of these invariants hold:
+--
+-- * Arrange that the in-scope set really is all the things in scope
+--
+-- * Arrange that it's the free vars of the range of the substitution
+--
+-- * Make it empty, if you know that all the free vars of the substitution are fresh, and hence can't possibly clash
+data Subst
+  = Subst InScopeSet  -- Variables in in scope (both Ids and TyVars) /after/
+                      -- applying the substitution
+          IdSubstEnv  -- Substitution from NcIds to CoreExprs
+          TvSubstEnv  -- Substitution from TyVars to Types
+          CvSubstEnv  -- Substitution from CoVars to Coercions
+
+        -- INVARIANT 1: See #in_scope_invariant#
+        -- This is what lets us deal with name capture properly
+        -- It's a hard invariant to check...
+        --
+        -- INVARIANT 2: The substitution is apply-once; see Note [Apply once] with
+        --              Types.TvSubstEnv
+        --
+        -- INVARIANT 3: See Note [Extending the Subst]
+
+{-
+Note [Extending the Subst]
+~~~~~~~~~~~~~~~~~~~~~~~~~~
+For a core Subst, which binds Ids as well, we make a different choice for Ids
+than we do for TyVars.
+
+For TyVars, see Note [Extending the TCvSubst] with Type.TvSubstEnv
+
+For Ids, we have a different invariant
+        The IdSubstEnv is extended *only* when the Unique on an Id changes
+        Otherwise, we just extend the InScopeSet
+
+In consequence:
+
+* If all subst envs are empty, substExpr would be a
+  no-op, so substExprSC ("short cut") does nothing.
+
+  However, substExpr still goes ahead and substitutes.  Reason: we may
+  want to replace existing Ids with new ones from the in-scope set, to
+  avoid space leaks.
+
+* In substIdBndr, we extend the IdSubstEnv only when the unique changes
+
+* If the CvSubstEnv, TvSubstEnv and IdSubstEnv are all empty,
+  substExpr does nothing (Note that the above rule for substIdBndr
+  maintains this property.  If the incoming envts are both empty, then
+  substituting the type and IdInfo can't change anything.)
+
+* In lookupIdSubst, we *must* look up the Id in the in-scope set, because
+  it may contain non-trivial changes.  Example:
+        (/\a. \x:a. ...x...) Int
+  We extend the TvSubstEnv with [a |-> Int]; but x's unique does not change
+  so we only extend the in-scope set.  Then we must look up in the in-scope
+  set when we find the occurrence of x.
+
+* The requirement to look up the Id in the in-scope set means that we
+  must NOT take no-op short cut when the IdSubst is empty.
+  We must still look up every Id in the in-scope set.
+
+* (However, we don't need to do so for expressions found in the IdSubst
+  itself, whose range is assumed to be correct wrt the in-scope set.)
+
+Why do we make a different choice for the IdSubstEnv than the
+TvSubstEnv and CvSubstEnv?
+
+* For Ids, we change the IdInfo all the time (e.g. deleting the
+  unfolding), and adding it back later, so using the TyVar convention
+  would entail extending the substitution almost all the time
+
+* The simplifier wants to look up in the in-scope set anyway, in case it
+  can see a better unfolding from an enclosing case expression
+
+* For TyVars, only coercion variables can possibly change, and they are
+  easy to spot
+-}
+
+
+
+*)
